ExprEval/Steps.lean
@@ -1,14 +1,41 @@
 import ExprEval.Expr
-import ExprEval.ArStepLemmas
 
-def eval_bool (val: V -> Int) (e: BoolExpr V): Bool :=
-    match e with
-    | BoolExpr.Const b => b
-    | BoolExpr.Less l r =>  (eval V val l) < (eval V val r)
-    | BoolExpr.Eq l r => (eval V val l) == (eval V val r)
-    | BoolExpr.Not e => not (eval_bool val e)
-    | BoolExpr.And l r => if eval_bool val l then eval_bool val r else false
-    | BoolExpr.Or l r => if eval_bool val l then true else eval_bool val r
+variable (V: Type)
+
+-- Small steps semantic for arithmetic expressions
+mutual
+inductive ArStep: (val: V -> Int) -> (ArExpr V) -> (ArExpr V) -> Prop where
+    | getVarValue (var: V) :
+        ArStep
+            val
+            (ArExpr.Var var)
+            (ArExpr.Const (val var))
+    | addConstConst(n₁ n₂: Int) :
+        ArStep
+            val
+            (ArExpr.Add (ArExpr.Const n₁) (ArExpr.Const n₂))
+            (ArExpr.Const (n₁ + n₂))
+    | subConstConst(n₁ n₂: Int) :
+        ArStep
+            val
+            (ArExpr.Sub (ArExpr.Const n₁) (ArExpr.Const n₂))
+            (ArExpr.Const (n₁ - n₂))
+    | mulConstConst(n₁ n₂: Int) :
+        ArStep
+            val
+            (ArExpr.Mul (ArExpr.Const n₁) (ArExpr.Const n₂))
+            (ArExpr.Const (n₁ * n₂))
+    | addLeft (e₁ e₁' e₂) : ArStep val e₁ e₁' -> ArStep val (ArExpr.Add e₁ e₂) (ArExpr.Add e₁' e₂)
+
+    | subLeft (e₁ e₁' e₂) : ArStep val e₁ e₁' -> ArStep val (ArExpr.Sub e₁ e₂) (ArExpr.Sub e₁' e₂)
+
+    | mulLeft (e₁ e₁' e₂) : ArStep val e₁ e₁' -> ArStep val (ArExpr.Mul e₁ e₂) (ArExpr.Mul e₁' e₂)
+
+    | addRight (n: Int) (e₂ e₂': ArExpr V) : ArStep val e₂ e₂' -> ArStep val (ArExpr.Add (ArExpr.Const n) e₂)  (ArExpr.Add (ArExpr.Const n) e₂')
+
+    | subRight (n: Int) (e₂ e₂': ArExpr V) : ArStep val e₂ e₂' -> ArStep val (ArExpr.Sub (ArExpr.Const n) e₂)  (ArExpr.Sub (ArExpr.Const n) e₂')
+    | mulRight (n: Int) (e₂ e₂': ArExpr V) : ArStep val e₂ e₂' -> ArStep val (ArExpr.Mul (ArExpr.Const n) e₂)  (ArExpr.Mul (ArExpr.Const n) e₂')
+
 
 inductive BoolStep: (val: V -> Int) -> (BoolExpr V) -> (BoolExpr V) -> Prop where
     | notIsBoolNot (b: Bool): BoolStep val
@@ -39,22 +66,22 @@ inductive BoolStep: (val: V -> Int) -> (BoolExpr V) -> (BoolExpr V) -> Prop wher
         (BoolExpr.Eq (ArExpr.Const n₁) (ArExpr.Const n₂))
         (BoolExpr.Const false)
     | lessArStepLeft (e₁ e₁' e₂: ArExpr V):
-        ArStep V val e₁ e₁' ->
+        ArStep val e₁ e₁' ->
             BoolStep val
                 (BoolExpr.Less e₁ e₂)
                 (BoolExpr.Less e₁' e₂)
     | eqArStepLeft (e₁ e₁' e₂: ArExpr V):
-        ArStep V val e₁ e₁' ->
+        ArStep val e₁ e₁' ->
             BoolStep val
                 (BoolExpr.Eq e₁ e₂)
                 (BoolExpr.Eq e₁' e₂)
      | lessArStepRight (e₁ e₂ e₂': ArExpr V):
-        ArStep V val e₂ e₂' ->
+        ArStep val e₂ e₂' ->
             BoolStep val
                 (BoolExpr.Less e₁ e₂)
                 (BoolExpr.Less e₁ e₂')
     | eqArStepRight (e₁ e₂ e₂': ArExpr V):
-        ArStep V val e₂ e₂' ->
+        ArStep val e₂ e₂' ->
             BoolStep val
                 (BoolExpr.Eq e₁ e₂)
                 (BoolExpr.Eq e₁ e₂')
@@ -72,7 +99,12 @@ inductive BoolStep: (val: V -> Int) -> (BoolExpr V) -> (BoolExpr V) -> Prop wher
         BoolStep val e e' -> BoolStep val
             (BoolExpr.Not e)
             (BoolExpr.Not e')
+end
 
-def BoolStepStar (V: Type) := StepStar (Step := BoolStep) V
-def BoolStepStar.refl {V: Type} (val: V -> Int) := StepStar.refl (Step := BoolStep) val
-def BoolStepStar.trans {V: Type} {val: V -> Int} e₁ e₂ e₃ := StepStar.trans e₁ e₂ e₃ (Step := BoolStep) (val := val)
+def ArStepStar (V: Type) := StepStar (Step := ArStep V) V
+def ArStepStar.refl {V: Type} (val: V -> Int) := StepStar.refl (Step := ArStep V) val
+def ArStepStar.trans {V: Type} {val: V -> Int} e₁ e₂ e₃ := StepStar.trans e₁ e₂ e₃ (Step := ArStep V) (val := val)
+
+def BoolStepStar (V: Type) := StepStar (Step := BoolStep V) V
+def BoolStepStar.refl {V: Type} (val: V -> Int) := StepStar.refl (Step := BoolStep V) val
+def BoolStepStar.trans {V: Type} {val: V -> Int} e₁ e₂ e₃ := StepStar.trans e₁ e₂ e₃ (Step := BoolStep V) (val := val)
