ExprEval/Basic.lean
@@ -1,47 +1,45 @@
-import ExprEval.Arithmetic
-import ExprEval.Boolean
-
-import ExprEval.ArStepLemmas
-import ExprEval.BoolStepLemmas
+import ExprEval.Steps
+import ExprEval.Lemmas
 
 variable (V: Type)
 
 theorem eval_soundness (e: ArExpr V) (v: Int) :
     ArStepStar V val e (ArExpr.Const v) -> eval V val e = v := by
-    exact arstepstar_preserves_eval _ _ _
+    intro h
+    exact arstepstar_preserves_eval _ _ h
 
 
 theorem eval_completeness (e: ArExpr V) : ArStepStar V val e (ArExpr.Const (eval V val e)) := by
-    induction e with
+    cases e with
     | Const x =>
         simp [eval]
         exact ArStepStar.refl _ _
-    | Add e₁ e₂ ih1 ih2 =>
-        -- ih1 : ArStepStar e₁ (ArExpr.Const (eval e₁))
-        -- ih2 : ArStepStar e₂ (ArExpr.Const (eval e₂))
+    | Add e₁ e₂ =>
+        have ih1 := eval_completeness e₁ (val := val)
+        have ih2 := eval_completeness e₂ (val := val)
         simp [eval]
-        have a := arstepstar_add_left _ _ _ e₂ ih1
-        have b := arstepstar_add_right _ (eval V val e₁) e₂ _ ih2
+        have a := arstepstar_add_left _ _ e₂ ih1
+        have b := arstepstar_add_right (eval V val e₁) e₂ _ ih2
         have c := ArStep.addConstConst (val := val) (eval V val e₁) (eval V val e₂)
         have d := ArStepStar.trans _ _ _ c (ArStepStar.refl _ (ArExpr.Const (eval V val e₁ + eval V val e₂)))
         have e := chasles_step_star _ a (chasles_step_star _ b d)
         exact e
-    | Sub e₁ e₂ ih1 ih2 =>
-        -- ih1 : ArStepStar e₁ (ArExpr.Const (eval e₁))
-        -- ih2 : ArStepStar e₂ (ArExpr.Const (eval e₂))
+    | Sub e₁ e₂ =>
+        have ih1 := eval_completeness e₁ (val := val)
+        have ih2 := eval_completeness e₂ (val := val)
         simp [eval]
-        have a := arstepstar_sub_left _ _ _ e₂ ih1
-        have b := arstepstar_sub_right _ (eval V val e₁) e₂ _ ih2
+        have a := arstepstar_sub_left _ _ e₂ ih1
+        have b := arstepstar_sub_right (eval V val e₁) e₂ _ ih2
         have c := ArStep.subConstConst (val := val) (eval V val e₁) (eval V val e₂)
         have d := ArStepStar.trans _ _ _ c (ArStepStar.refl _ (ArExpr.Const  (eval V val e₁ - eval V val e₂)))
         have e := chasles_step_star _ a (chasles_step_star _ b d)
         exact e
-    | Mul e₁ e₂ ih1 ih2 =>
-        -- ih1 : ArStepStar e₁ (ArExpr.Const (eval e₁))
-        -- ih2 : ArStepStar e₂ (ArExpr.Const (eval e₂))
+    | Mul e₁ e₂ =>
+        have ih1 := eval_completeness e₁ (val := val)
+        have ih2 := eval_completeness e₂ (val := val)
         simp [eval]
-        have a := arstepstar_mul_left _ _ _ e₂ ih1
-        have b := arstepstar_mul_right _ (eval V val e₁) e₂ _ ih2
+        have a := arstepstar_mul_left _ _ e₂ ih1
+        have b := arstepstar_mul_right (eval V val e₁) e₂ _ ih2
         have c := ArStep.mulConstConst (val := val) (eval V val e₁) (eval V val e₂)
         have d := ArStepStar.trans _ _ _ c (ArStepStar.refl _ (ArExpr.Const (eval  V val e₁ * eval V val e₂)))
         have e := chasles_step_star _ a (chasles_step_star _ b d)
@@ -53,24 +51,27 @@ theorem eval_completeness (e: ArExpr V) : ArStepStar V val e (ArExpr.Const (eval
         exact ArStepStar.trans (val := val) _ _ _ a b
 
 theorem eval_bool_soundness (e: BoolExpr V) (b: Bool) :
-    BoolStepStar V val e (BoolExpr.Const b) -> eval_bool val e = b := by
+    BoolStepStar V val e (BoolExpr.Const b) -> eval_bool V val e = b := by
     intro h
     exact boolstepstar_preserves_eval_bool _ _ h
 
-theorem eval_bool_completeness (e: BoolExpr V): BoolStepStar V val e (BoolExpr.Const (eval_bool val e)) := by
-    induction e with
+theorem eval_bool_completeness (e: BoolExpr V): BoolStepStar V val e (BoolExpr.Const (eval_bool V val e)) := by
+    cases e with
     | Const b =>
         simp [eval_bool]
         apply BoolStepStar.refl
-    | Not e ihn =>
+    | Not e =>
         simp [eval_bool]
+        have ihn := eval_bool_completeness e (val := val)
         have h := BoolStepStar.notStep e _ ihn
-        have h1 := BoolStep.notIsBoolNot (eval_bool val e) (val := val)
+        have h1 := BoolStep.notIsBoolNot (eval_bool V val e) (val := val)
         have h2 := (step_to_stepstar V h1)
         apply chasles_step_star V h h2
-    | And l r l_step r_step =>
+    | And l r =>
+        have l_step := eval_bool_completeness l (val := val)
+        have r_step := eval_bool_completeness r (val := val)
         simp [eval_bool]
-        by_cases h: (eval_bool val l)
+        by_cases h: (eval_bool V val l)
         .   simp [and]
             rw [h]
             simp
@@ -88,9 +89,11 @@ theorem eval_bool_completeness (e: BoolExpr V): BoolStepStar V val e (BoolExpr.C
             have h2 := BoolStep.andLeftShortCircuit r (val := val)
             have h3 := step_to_stepstar V h2
             exact chasles_step_star V h1 h3
-    | Or l r l_step r_step =>
+    | Or l r =>
+        have l_step := eval_bool_completeness l (val := val)
+        have r_step := eval_bool_completeness r (val := val)
         simp [eval_bool]
-        by_cases h: (eval_bool val l)
+        by_cases h: (eval_bool V val l)
         .   rw [h]
             rw [h] at l_step
             simp [or]
